\marker{Discrete}: \textbf{finite} or \textbf{countably infinite}

\marker{Probability Mass Function (p.m.f.)} \(p_X(x)\):
\begin{equation*}
p_X(x) = \begin{cases}P(X=x), & \text{if }x = x_1, x_2, \cdots \\ 0, & 
\text{otherwise}.\end{cases}
\end{equation*}
Note that \(\sum\limits_{i=1}^{\infty}p_X(x_i) = 1\).

\marker{Cumulative Distribution Function (c.d.f.)} \(F_X(x)\):
\[F_X(x) = P(X \leq x)\]

\marker{Expectation}: \(X\) \textbf{discrete} with \textbf{p.m.f.}
\(p_X\) \tf \textbf{expectation}
\begin{equation*}
  E(X) := \sum\limits_{x}xp_X(x).
\end{equation*}
\marker{Tail Sum Formula}: \(X \in \mathbb{Z}^+\) \tf
\begin{equation*}
E(X) = \sum\limits_{k=1}^{\infty}P(X \geq k) = 
\sum\limits_{k=0}^{\infty}P(X > k).
\end{equation*}

\marker{Expectation of a Function}: \(X\) \textbf{discrete} with \(p_X\),
\(g\):
\begin{equation*}
  E[g(X)] = \sum_i g(x_i)p_X(x_i) = \sum_x g(x)p_X(x).
\end{equation*}
\[E[aX + b] = aE(X)+ b.\]
\marker{Variance} Let \(\mu := E(X)\), i.e. \textbf{mean} of \(X\),
\[ \operatorname{Var}\left(X\right)=E[(X-\mu)^2]. \]
\marker{Zero Variance} If \(\operatorname{Var}\left(X\right) = 0\), then the
random variable \(X\) is a constant.
\marker{Standard Deviation} 
\(\sigma_X\) or \(\operatorname{SD}\left(X\right)\):
\(\sigma_X := \sqrt{\operatorname{Var}\left(X\right)}.\)

\marker{Scaling and shifting}: 
\begin{multicols}{2}
\begin{itemize}
  \item \(\operatorname{Var}\left(aX+b\right)=a^2\operatorname{Var}
    \left(X\right)\);
  \item \(\operatorname{SD}\left(aX+b\right)=|a|\operatorname{SD}
    \left(X\right)\).
\end{itemize}
\end{multicols}

\marker{Properties of d.f.}:
\begin{itemize}
  \item \(F_X\) \textbf{non-decreasing} \tf \(F_X(a) \leq F_X(b)\);
  \item \(\lim\limits_{b\rightarrow \infty}F_X(b) = 1\), and
    \(\lim\limits_{b\rightarrow -\infty}F_X(b) = 0\);
  \item \(F_X\) has \textbf{left limits}, i.e. \(\lim\limits_{x\rightarrow
    b^-}F_X(x)\) exists for all \(b\in \mathbb{R}\);
  \item \(F_X\) is \textbf{right continuous}, i.e. \(\forall b \in
    \mathbb{R}\), \(\lim\limits_{x\rightarrow b^+}F_X(x) = F_X(b)\).
\end{itemize}

\marker{Useful Calculations}:
\begin{enumerate}
  \item \(P\) from \textbf{d.f.}:
  \begin{itemize}
    \item \(P(a<X\leq b)=F_X(b) - F_X(a)\);
    \item \(P(X=a)=F_X(a)-F_X(a^-)\), where 
      \(F_X(a^-)=\lim\limits_{x\rightarrow a^-}F_X(x)\).
    \item \(\begin{aligned}
        P(a \leq X \leq b) &= P(X = a) + P(a < X \leq b) \\ &= F_X(b)-F_X(a^-).
    \end{aligned}\)
  \end{itemize}
  \item \(P\) from \textbf{PMF}: \(P(A) = \sum_{x\in A}p_X(x)\);
  \item \textbf{p.m.f.} from \textbf{d.f.}: \(p_X(x) = F_X(x) - F_X(x^-)\);
  \item \textbf{d.f.} from \textbf{p.m.f.}: \(F_X(x) = \sum_{y\leq x}p_X(y)\).
\end{enumerate}

